wip

theories/CombinatoryLogic/L_CBN_Interpreter.v
@@ -56,6 +56,8 @@ Inductive halt_cbn : list eterm -> eterm -> Prop :=
 (* most easy to simulate halt_cbn 
 halt_cbn [t1 .. tn] ctx t means that (t t1 .. tn) halts in context ctx (terms for free variables)
 *)
+(* actual krivine machine
+https://en.wikipedia.org/wiki/Krivine_machine *)
 Inductive halt_cbn : list eterm -> list eterm -> term -> Prop :=
   | halt_var_0 ts ctx t ctx' :
       halt_cbn ts ctx t ->
@@ -64,7 +66,7 @@ Inductive halt_cbn : list eterm -> list eterm -> term -> Prop :=
       halt_cbn ts ctx (var n) ->
       halt_cbn ts (t::ctx) (var (S n))
   | halt_app ts ctx s t :
-      halt_cbn ((closure ctx t) :: ts) ctx s ->
+      halt_cbn ((closure ctx t)::ts) ctx s ->
       halt_cbn ts ctx (app s t)
   | halt_lam_ts t ts ctx s :
       halt_cbn ts (t::ctx) s ->
@@ -79,7 +81,11 @@ Lemma halt_cbnE ts ctx u : halt_cbn ts ctx u ->
       | [] => False
       | (closure ctx' t')::_ => halt_cbn ts ctx' t'
       end
-  | var (S n) => True
+  | var (S n) => 
+      match ctx with
+      | [] => False
+      | _::ctx' => halt_cbn ts ctx' (var n)
+      end
   | app s t => halt_cbn ((closure ctx t) :: ts) ctx s
   | lam s =>
       match ts with
@@ -118,30 +124,511 @@ Proof.
   move=> t ctx IH k s. by rewrite IH.
 Qed.
 
+(*
+Forall (fun t => 
+(exists t', t = closure (map (closure []) ctx) t') \/ 
+(exists t', t = closure [] (subst_list 0 ctx t'))) ts ->
+*)
 
-Lemma asd ts s ctx :
-  Forall (fun t => 
-    (exists t', t = closure (map (closure []) ctx) t') \/ 
-    (exists t', t = closure [] (subst_list 0 ctx t'))) ts ->
-  halt_cbn ts [] (subst_list 0 ctx s) ->
-  halt_cbn ts (map (closure []) ctx) s.
+Lemma Forall2_consE {X : Type} {P : X -> X -> Prop} {x1 l1 x2 l2} : 
+  Forall2 P (x1::l1) (x2::l2) -> P x1 x2 /\ Forall2 P l1 l2.
+Proof. move=> H. by inversion H. Qed.
+
+Inductive ctx_size : nat -> list eterm -> Prop :=
+  | ctx_size_nil : ctx_size 0 []
+  | ctx_size_cons n ctx1 m ctx2 t :
+      ctx_size n ctx1 -> ctx_size m ctx2 -> ctx_size (1+n+m) ((closure ctx1 t)::ctx2).
+
+Inductive closureT (P : list eterm -> Type) : eterm -> Type :=
+  | closureT_closure ctx t : P ctx -> closureT P (closure ctx t).
+
+Inductive contextT (P : eterm -> Type) : list eterm -> Type :=
+  | contextT_nil : contextT P []
+  | contextT_cons u ctx : P u -> contextT P ctx -> contextT P (u::ctx).
+
+Definition contextTI (P : eterm -> Type) : (forall u, P u) -> forall ctx, contextT P ctx.
 Proof.
-  elim: s ts ctx.
+  move=> H. elim.
+  - apply: contextT_nil.
+  - move=> ???. apply: contextT_cons. apply: H. done.
+Defined.
+
+Inductive Plist {X : Type} (P : X -> Type) : list X -> Type :=
+  | Plist_nil : Plist P []
+  | Plist_cons x l : P x -> Plist P l -> Plist P (x::l).
+
+Unset Implicit Arguments.
+
+Definition Flist {X : Type} (P : X -> Type) (f : forall l, P l) (l : list X) : Plist P l.
+Proof.
+  elim: l.
+  - apply: Plist_nil.
+  - move=> x l IH. apply: Plist_cons.
+    + apply: f.
+    + apply: IH.
+Defined.
+
+Definition closureTI (P : eterm -> Type) : (forall ctx t, Plist P ctx -> P (closure ctx t)) -> forall u, P u :=
+  fun H => fix f (u : eterm) : P u :=
+  match u with
+  | closure ctx t => H ctx t (Flist P f ctx)
+  end.
+
+(* using unary parametricity similar to rosetrees *)
+Fixpoint closure_rect (P : eterm -> Type) (H : forall ctx t, Plist P ctx -> P (closure ctx t)) u : P u :=
+  match u with
+  | closure ctx t => H ctx t (Flist P (closure_rect P H) ctx)
+  end.
+
+Fixpoint term_size (t : term) : nat :=
+  match t with
+  | var n => n
+  | app s t => 1 + term_size s + term_size t
+  | lam s => 1 + term_size s
+  end.
+
+Definition eterm_size (u : eterm) : nat.
+Proof.
+  refine (closure_rect (fun=> nat) _ u).
+  intros ?? H. induction H.
+  - exact (term_size t).
+  - exact (1 + p + IHPlist).
+Defined.
+
+Definition context_size (ctx : list eterm) : nat.
+Proof.
+  refine (closure_rect (fun=> nat) _ (closure ctx (var 0))).
+  intros ?? H. induction H.
+  - exact 0.
+  - exact (1 + p + IHPlist).
+Defined.
+
+Lemma context_size_cons ctx1 t ctx2 :
+  context_size ((closure ctx1 t)::ctx2) = 1 + (context_size ctx1) + (context_size ctx2).
+Proof. done. Qed.
+
+
+(* induction/recursion principle wrt. a decreasing measure f *)
+(* example: elim /(measure_rect length) : l. *)
+Lemma measure_rect {X : Type} (f : X -> nat) (P : X -> Type) : 
+  (forall x, (forall y, f y < f x -> P y) -> P x) -> forall (x : X), P x.
+Proof.
+  exact: (well_founded_induction_type (Wf_nat.well_founded_lt_compat X f _ (fun _ _ => id)) P).
+Qed.
+
+
+Lemma ind_on_der ts1 ts2 ctx1 ctx2 s1 s2:
+  Forall2 (fun t1 t2 => flatten t1 = flatten t2) ts1 ts2 ->
+  flatten (closure ctx1 s1) = flatten (closure ctx2 s2) ->
+  halt_cbn ts1 ctx1 s1 ->
+  halt_cbn ts2 ctx2 s2.
+Proof.
+  move=> ++ H. elim: H ts2 ctx2 s2; clear ts1 ctx1 s1.
+  - move=> ts ctx t ctx' ? IH ts2 ctx2 s2.
+    move=> ? /= ?.
+    have : flatten (closure ctx t) = flatten (closure ctx2 s2) by admit.
+    move=> ?.
+    by apply: (IH ts2 ctx2 s2).
+  - move=> ts1 ctx1 n t ? IH ts2 ctx2 s2 ?.
+    move=> /= ?.
+    apply: (IH ts2 ctx2 s2).
+    done.
+    admit. (* by closedness *)
+  - move=> ts1 ctx1 s t ? IH ts2 ctx2 s2 ?.
+    move=> /=. rewrite subst_list_app.
+    (* maybe here induction on ctx2 size for var elimination? *)
+    case: s2.
+    + move=> [|n]; last by admit.
+      case: ctx2 => [|t2 ctx2]; first done.
+      move=> /=.
+      have ->: subst_list 1 (map flatten ctx2) (flatten t2) = flatten t2.
+      admit.
+      case: t2 => ctx' t2.
+      have : exists t21 t22, t2 = app t21 t22 by admit.
+      (* variable case problematic? needs more recursion? *)
+      move=> [t21] [t22] -> /=.
+      rewrite subst_list_app.
+      move=> [??]. apply: halt_var_0. apply: halt_app.
+      apply: IH.
+      admit. admit. (* looks good *)
+    + move=> ??.       rewrite subst_list_app.
+    move=> [??].  apply: halt_app.
+    apply: IH. admit. admit. (* looks good *)
+    + admit.
+  - move=> t1 ts1 ctx1 s1 ? IH ts2 ctx2 s2.
+    case: ts2 => [|t2 ts2].
+    { move=> H. inversion H. }
+    move=> /Forall2_consE [??].
+    case: s2.
+    + move=> [|n]; last admit.
+      move=> /=.
+      case: ctx2 => [|[ctx2' t2'] ctx2]; first admit.
+      move=> /= ?.
+      apply: halt_var_0.
+      have : exists t2'', t2' = lam t2'' by admit.
+      move=> [? ->].
+      apply: halt_lam_ts.
+      apply: IH.
+      done.
+      admit. (* looks promising *)
+    + admit.
+    + move=> s2 /=. rewrite !subst_list_lam.
+      move=> [?].       apply: halt_lam_ts.
+      apply: IH. done.
+      admit.
+  - admit. (* similar *)
+
+
+
+  elim /(measure_rect context_size): ctx1 s1 ts1 s2 ts2 ctx2.
+  move=> ctx1 IH s1.
+  elim: s1 ctx1 IH.
+  - move=> [|n] [|[ctx' t'] ctx1].
+    + by move=> ? > ?? /halt_cbnE.
+    + move=> IH ts1 s2 ts2 ctx2 /= ??.
+      move=> /halt_cbnE. apply: IH.
+      * move=> /=. rewrite context_size_cons. lia.
+      * done.
+      * admit. (* doable *)
+    + by move=> ? > ?? /halt_cbnE.
+    + move=> IH ts1 s2 ts2 ctx2 /= ??.
+      move=> /halt_cbnE. apply: IH.
+      * move=> /=. rewrite context_size_cons. lia.
+      * done.
+      * admit. (* doable *)
+  - move=> s'1 IH1. s'2 IH2 ts1 s2 ts2 ctx1 ctx2 /=.
+    move=> Hts. rewrite subst_list_app.
+    case: s2.
+    + admit.
+    + move=> s''1 s''2. rewrite subst_list_app.
+      move=> [] /IH1 {}IH1 ?.
+      move=> /halt_cbnE ?. apply: halt_app.
+      apply: IH1; [|eassumption].
+      by  constructor.
+    + move=> ?. by rewrite subst_list_lam.
+  - move=> s'1 IH ts1 s2 ts2 ctx1 ctx2 /=. case: s2.
+    + admit.
+    + move=> >. by rewrite subst_list_app subst_list_lam.
+    + move=> s'2 Hts. rewrite !subst_list_lam.
+      move=> [?].
+      move: ts2 ts1 Hts => [|t1 ts1] [|t2 ts2].
+      * move=> *. by apply: halt_lam.
+      * move=> *. by apply: halt_lam.
+      * move=> H. by inversion H.
+      * move=> /Forall2_consE [? ?] /halt_cbnE H'. apply: halt_lam_ts.
+        move: H'. apply: IH.
+        ** done.
+        ** move=> /=. admit. (* doable with well-formedness *)
+*)
+
+(* interpreter *)
+Definition many_app s ts := fold_left app ts s.
+
+
+Lemma halt_cbn_closed {ts ctx1 ctx2 s} : closed s -> halt_cbn ts ctx1 s -> halt_cbn ts ctx2 s.
+Proof. Admitted.
+
+Definition mk_O := lam (lam (var 1)).
+Definition mk_S (n : term) := lam (lam (app (var 0) n)).
+Fixpoint enc_nat (n : nat) : term :=
+  match n with
+  | 0 => mk_O
+  | (S n) => mk_S (enc_nat n)
+  end.
+
+Lemma enc_nat_closed n : closed (enc_nat n).
+Proof.
+  elim: n; first done.
+  move=> n IH m t /=. by rewrite IH.
+Qed.
+
+Definition rho (s : term) := 
+  let C := lam (lam (app (var 0) (lam (app (app (app (var 2) (var 2)) (var 1)) (var 0))))) in
+  lam (app (app (app C C) s) (var 0)).
+
+Lemma rho_spec s t ts : closed s -> 
+  halt_cbn (t::ts) [] (app s (rho s)) ->
+  halt_cbn (t::ts) [] (rho s).
+Proof.
+  move=> Hs. rewrite /rho.
+  move=> /halt_cbnE H'.
+  do ? constructor.
+Admitted.
+
+(* given n m, if m = n then s else t *)
+Definition nat_beq s t := rho (lam (lam (lam (
+  (* [m n nat_beq] *) many_app (var 1) [
+      many_app (var 0) [s; lam t];
+      lam (many_app (var 1) [t; lam (app (app (var 4) (var 1)) (var 0))])
+  ])))).
+
+Lemma nat_beq_closed {s t} : closed s -> closed t -> closed (nat_beq s t).
+Proof. Admitted. 
+
+(*
+Lemma subst_nat_beq {s t} n u : subst (nat_beq s t) n u = nat_beq (subst s n u) (subst t n u).
+Proof.
+  rewrite /nat_beq /=.
+*)
+
+Lemma halt_cbn_app_closed_r {ts ctx s t} : 
+  closed t ->
+  halt_cbn ((closure [] t)::ts) ctx s ->
+  halt_cbn ts ctx (app s t).
+Proof. Admitted.
+
+Lemma halt_cbn_app_var_r {ts ctx s t n} : 
+  nth_error ctx n = Some t ->
+  halt_cbn (t::ts) ctx s ->
+  halt_cbn ts ctx (app s (var n)).
+Proof. Admitted.
+
+Arguments halt_cbn_app_var_r {ts ctx s t n} & _.
+
+Lemma nat_beq_spec s t n m ts : closed s -> closed t ->
+  halt_cbn ts [] (if Nat.eqb n m then s else t) ->
+  halt_cbn ts [] (app (app (nat_beq s t) (enc_nat n)) (enc_nat m)).
+Proof.
+  move=> Hs Ht.
+  elim: n m.
+  - move=> [|m] /= H'.
+    + do ? constructor. by apply: (halt_cbn_closed Hs H').
+    + do ? constructor. by apply: (halt_cbn_closed Ht H').
+  - move=> n IH [|m] /= H'.
+    + do ? constructor. by apply: (halt_cbn_closed Ht H').
+    + move: H' => /IH /halt_cbnE /halt_cbnE H'.
+      do 2 constructor.
+      apply: rho_spec. { move=> n' t' /=. by rewrite Hs Ht. }
+      rewrite -/(nat_beq s t).
+      move: (nat_beq s t) H' => ? H'.
+      do ?
+      first [
+        apply: (halt_cbn_app_closed_r (enc_nat_closed _)) |
+        apply: halt_cbn_app_var_r; [apply: erefl|] |
+        constructor].
+      done.
+Qed.
+
+Definition mk_var (n : term) := lam (lam (lam (app (var 2) n))).
+Definition mk_app (s t : term) := lam (lam (lam (app (app (var 1) s) t))).
+Definition mk_lam (s : term) := lam (lam (lam (app (var 0) s))).
+
+Fixpoint enc_term (s : term) : term :=
+  match s with
+  | var n => mk_var (enc_nat n)
+  | app s t => mk_app (enc_term s) (enc_term t)
+  | lam s => mk_lam (enc_term s)
+  end.
+
+Lemma enc_term_closed s : closed (enc_term s).
+Proof.
+  elim: s.
+  - move=> ??? /=. by rewrite enc_nat_closed.
+  - move=> s IHs t IHt ?? /=. by rewrite IHs IHt.
+  - move=> s IH ?? /=. by rewrite IH.
+Qed.
+
+(* substitute s n t *)
+Definition substituter t := rho (lam (lam (lam (
+    (* [n s substituter] *) 
+  many_app (var 1) [
+    (* case s = var n *)     lam (app (app (nat_beq (var 0) (var 2)) (var 1)) t);
+    (* case s = app s' t' *) (lam (lam (mk_app 
+      (app (app (app (var 4) (var 3)) (var 2)) (var 1))
+      (app (app (app (var 4) (var 3)) (var 2)) (var 0)))));
+    (* case s = lam s' *) (lam (mk_lam
+      (app (app (app (var 3) (var 2)) (mk_S (var 1))) (var 0))
+    ))])))).
+  
+Lemma substituter_spec s t n ts : closed t ->
+  halt_cbn ts [] (enc_term (subst s n t)) ->
+  halt_cbn ts [] (app (app (substituter t) (enc_term s)) (enc_nat n)).
+Proof.
+  move=> Ht.
+  elim: s n.
+  - move=> m n H'.
+    do 2 constructor.
+    apply: rho_spec. { move=> n' t' /=. by rewrite Ht. }
+    rewrite -/(substituter t). move: (substituter _) => ?.
+    Opaque nat_beq.
+    do ?
+    first [
+      apply: (halt_cbn_app_closed_r (enc_nat_closed _)) |
+      apply: halt_cbn_app_var_r; [apply: erefl|] |
+      constructor].
+    done.
+
+  - move=> n IH [|m] /= H'.
+    + do ? constructor. by apply: (halt_cbn_closed Ht H').
+    + move: H' => /IH /halt_cbnE /halt_cbnE H'.
+      do 2 constructor.
+      apply: rho_spec. { move=> n' t' /=. by rewrite Hs Ht. }
+      rewrite -/(nat_beq s t).
+      move: (nat_beq s t) H' => ? H'.
+      do ?
+      first [
+        apply: (halt_cbn_app_closed_r (enc_nat_closed _)) |
+        apply: halt_cbn_app_var_r; [apply: erefl|] |
+        constructor].
+      done.
+
+(* right direction, almost*
+Lemma asd ts1 ts2 ctx1 ctx2 s1 s2:
+  Forall2 (fun t1 t2 => flatten t1 = flatten t2) ts1 ts2 ->
+  flatten (closure ctx1 s1) = flatten (closure ctx2 s2) ->
+  halt_cbn ts1 ctx1 s1 ->
+  halt_cbn ts2 ctx2 s2.
+Proof.
+  elim /(measure_rect context_size): ctx1 s1 ts1 s2 ts2 ctx2.
+  move=> ctx1 IH s1.
+  elim: s1 ctx1 IH.
+  - move=> [|n] [|[ctx' t'] ctx1].
+    + by move=> ? > ?? /halt_cbnE.
+    + move=> IH ts1 s2 ts2 ctx2 /= ??.
+      move=> /halt_cbnE. apply: IH.
+      * move=> /=. rewrite context_size_cons. lia.
+      * done.
+      * admit. (* doable *)
+    + by move=> ? > ?? /halt_cbnE.
+    + move=> IH ts1 s2 ts2 ctx2 /= ??.
+      move=> /halt_cbnE. apply: IH.
+      * move=> /=. rewrite context_size_cons. lia.
+      * done.
+      * admit. (* doable *)
+  - move=> s'1 IH1. s'2 IH2 ts1 s2 ts2 ctx1 ctx2 /=.
+    move=> Hts. rewrite subst_list_app.
+    case: s2.
+    + admit.
+    + move=> s''1 s''2. rewrite subst_list_app.
+      move=> [] /IH1 {}IH1 ?.
+      move=> /halt_cbnE ?. apply: halt_app.
+      apply: IH1; [|eassumption].
+      by  constructor.
+    + move=> ?. by rewrite subst_list_lam.
+  - move=> s'1 IH ts1 s2 ts2 ctx1 ctx2 /=. case: s2.
+    + admit.
+    + move=> >. by rewrite subst_list_app subst_list_lam.
+    + move=> s'2 Hts. rewrite !subst_list_lam.
+      move=> [?].
+      move: ts2 ts1 Hts => [|t1 ts1] [|t2 ts2].
+      * move=> *. by apply: halt_lam.
+      * move=> *. by apply: halt_lam.
+      * move=> H. by inversion H.
+      * move=> /Forall2_consE [? ?] /halt_cbnE H'. apply: halt_lam_ts.
+        move: H'. apply: IH.
+        ** done.
+        ** move=> /=. admit. (* doable with well-formedness *)
+*)
+(*
+Lemma asd ts1 ts2 ctx1 ctx2 s1 s2:
+  Forall2 (fun t1 t2 => flatten t1 = flatten t2) ts1 ts2 ->
+  flatten (closure ctx1 s1) = flatten (closure ctx2 s2) ->
+  halt_cbn ts1 ctx1 s1 ->
+  halt_cbn ts2 ctx2 s2.
+Proof.
+  elim: s1 ts1 s2 ts2 ctx1 ctx2.
+  - move=> + ts1 s2 ts2 ctx1 ctx2 Hts.
+    admit.
+  - move=> s'1 IH1 s'2 IH2 ts1 s2 ts2 ctx1 ctx2 /=.
+    move=> Hts. rewrite subst_list_app.
+    case: s2.
+    + admit.
+    + move=> s''1 s''2. rewrite subst_list_app.
+      move=> [] /IH1 {}IH1 ?.
+      move=> /halt_cbnE ?. apply: halt_app.
+      apply: IH1; [|eassumption].
+      by  constructor.
+    + move=> ?. by rewrite subst_list_lam.
+  - move=> s'1 IH ts1 s2 ts2 ctx1 ctx2 /=. case: s2.
+    + admit.
+    + move=> >. by rewrite subst_list_app subst_list_lam.
+    + move=> s'2 Hts. rewrite !subst_list_lam.
+      move=> [?].
+      move: ts2 ts1 Hts => [|t1 ts1] [|t2 ts2].
+      * move=> *. by apply: halt_lam.
+      * move=> *. by apply: halt_lam.
+      * move=> H. by inversion H.
+      * move=> /Forall2_consE [? ?] /halt_cbnE H'. apply: halt_lam_ts.
+        move: H'. apply: IH.
+        ** done.
+        ** move=> /=. admit. (* doable with well-formedness *)
+
+
+(* same issue *)
+Lemma asd ts s (ctx : list eterm) t:
+  bound (S (length ctx)) s ->
+  halt_cbn ts ctx (subst s (length ctx) (flatten t)) ->
+  halt_cbn ts (ctx ++ [t]) s.
+Proof.
+  elim: s ts ctx t.
   - move=> [|n] ts ctx /=.
     + admit.
     + admit. (* closed *)
-  - move=> s1 IH1 s2 IH2 ts ctx Hts /=.
+  - move=> s1 IH1 s2 IH2 ts ctx t Hs /=.
+    move=> /halt_cbnE ?.
+    apply: halt_app. apply: IH1. admit. (* easy *)
+
+    have := (IH1 (s2 :: ts) (ctx1 ++ ctx2) ctx1 ctx2 erefl).
+    rewrite -Hctx. apply. done.
+
+(* still no *)
+Lemma asd ts s (ctx : list term) ctx1 ctx2:
+  ctx = ctx1 ++ ctx2 ->
+  halt_cbn 
+    (map (fun t => closure (map (closure []) ctx1) (subst_list (length ctx1) ctx2 t)) ts)
+    (map (closure []) ctx1) (subst_list (length ctx1) ctx2 s) ->
+  halt_cbn (map (closure (map (closure []) ctx)) ts) (map (closure []) ctx) s.
+Proof.
+  elim: s ts ctx ctx1 ctx2.
+  - move=> [|n] ts ctx /=.
+    + admit.
+    + admit. (* closed *)
+  - move=> s1 IH1 s2 IH2 ts ctx ctx1 ctx2 Hctx /=.
     rewrite subst_list_app.
+    move=> /halt_cbnE ?.
+    apply: halt_app.
+    have := (IH1 (s2 :: ts) (ctx1 ++ ctx2) ctx1 ctx2 erefl).
+    rewrite -Hctx. apply. done.
+    (*
     move=> /halt_cbnE /IH1 {}IH1.
     apply: halt_app.
 
-    admit. (* almost, needs subst in ts *)
-  - move=> s IH [|t' ts'] ctx /=.
+    admit. (* almost, needs subst in ts *)*)
+  - move=> s IH [|t' ts'] ctx ctx1 ctx2 Hctx /=.
     + move=> *. apply: halt_lam.
     + rewrite subst_list_lam. move=> /halt_cbnE ?.
       apply: halt_lam_ts.
-      apply: IH.
+      apply: (IH ts' (t' :: ctx) (t'::ctx1) ctx2).
+      * by rewrite Hctx.
+      * done.
 
+(* almost *)
+Lemma asd ts s ctx ctx1 ctx2:
+  ctx = ctx1 ++ ctx2 ->
+  halt_cbn (map (closure []) ts) (map (closure []) ctx1) (subst_list (length ctx1) ctx2 s) ->
+  halt_cbn (map (closure []) ts) (map (closure []) ctx) s.
+Proof.
+  elim: s ts ctx ctx1 ctx2.
+  - move=> [|n] ts ctx /=.
+    + admit.
+    + admit. (* closed *)
+  - move=> s1 IH1 s2 IH2 ts ctx ctx1 ctx2 Hctx /=.
+    rewrite subst_list_app.
+    move=> /halt_cbnE.
+    admit.
+    (*
+    move=> /halt_cbnE /IH1 {}IH1.
+    apply: halt_app.
+
+    admit. (* almost, needs subst in ts *)*)
+  - move=> s IH [|t' ts'] ctx ctx1 ctx2 Hctx /=.
+    + move=> *. apply: halt_lam.
+    + rewrite subst_list_lam. move=> /halt_cbnE ?.
+      apply: halt_lam_ts.
+      apply: (IH ts' (t' :: ctx) (t'::ctx1) ctx2).
+      * by rewrite Hctx.
+      * done.
+*)
 (* actually does not work because removing from ctx shifts indices and subst is plain *)
 (*
 Lemma asd ts s t ctx :
@@ -279,7 +766,7 @@ Admitted.
 
 
 
-Definition many_app s ts := fold_left app ts s.
+
 
 
 
