theories/CombinatoryLogic/Plotkin.v
@@ -1,0 +1,124 @@
+(* plotkin call by value call by name and lambda calculus *)
+
+From Undecidability Require L.L.
+Require Import List Lia.
+Import L.
+From Undecidability Require Import L.Util.L_facts.
+From Undecidability Require L.Computability.Seval.
+Require Import Relations.
+Require Import ssreflect ssrbool ssrfun.
+
+Inductive eterm := closure : list eterm -> term -> eterm.
+
+(* actual krivine machine
+https://en.wikipedia.org/wiki/Krivine_machine *)
+Inductive halt_cbn : list eterm -> list eterm -> term -> Prop :=
+  | halt_var_0 ts ctx t ctx' :
+      halt_cbn ts ctx t ->
+      halt_cbn ts ((closure ctx t)::ctx') (var 0)
+  | halt_var_S ts ctx n t :
+      halt_cbn ts ctx (var n) ->
+      halt_cbn ts (t::ctx) (var (S n))
+  | halt_app ts ctx s t :
+      halt_cbn ((closure ctx t)::ts) ctx s ->
+      halt_cbn ts ctx (app s t)
+  | halt_lam_ts t ts ctx s :
+      halt_cbn ts (t::ctx) s ->
+      halt_cbn (t::ts) ctx (lam s)
+  | halt_lam ctx s :
+      halt_cbn [] ctx (lam s).
+
+Lemma halt_cbnE ts ctx u : halt_cbn ts ctx u ->
+  match u with
+  | var 0 =>
+      match ctx with
+      | [] => False
+      | (closure ctx' t')::_ => halt_cbn ts ctx' t'
+      end
+  | var (S n) => 
+      match ctx with
+      | [] => False
+      | _::ctx' => halt_cbn ts ctx' (var n)
+      end
+  | app s t => halt_cbn ((closure ctx t) :: ts) ctx s
+  | lam s =>
+      match ts with
+      | [] => True
+      | t'::ts' => halt_cbn ts' (t'::ctx) s
+      end
+  end.
+Proof. by case. Qed.
+    
+(* left-most outer-most call-by-name *)
+Inductive step : term -> term -> Prop :=
+  | stepLam s t    : step (app (lam s) t) (subst s 0 t)
+  | stepApp s s' t : step s s' -> step (app s t) (app s' t).
+
+  (* function composition *)
+Definition funcomp {X Y Z} (g : Y -> Z) (f : X -> Y) :=
+  fun x => g (f x).
+
+(* stream cons *)
+Definition scons {X: Type} (x : X) (xi : nat -> X) :=
+  fun n => match n with | 0 => x | S n => xi n end.
+
+Fixpoint ren (xi : nat -> nat) (t : term) : term  :=
+  match t with
+  | var x => var (xi x)
+  | app s t => app (ren xi s) (ren xi t)
+  | lam t => lam (ren (scons 0 (funcomp S xi)) t)
+  end.
+
+Fixpoint cbv_cbn (t : term) : term :=
+  match t with
+  | var n => lam (app (var 0) (var (S n)))
+  | app s t => lam (app (ren S (cbv_cbn  s)) (lam (app (ren S (ren S (cbv_cbn t))) (lam (app (app (var 1) (var 0)) (var 2))))))
+  | lam s => lam (app (var 0) (ren S (lam (cbv_cbn s))))
+  end.
+
+Definition Psi (t : term) :=
+  match t with
+  | var n => var n
+  | app s t => app s t
+  | lam s => ren S (lam (cbv_cbn s))
+  end.
+
+Lemma subst_ren s k t : subst (ren S s) (S k) t = ren S (subst s k t).
+Proof. Admitted. (* needs closedness *)
+
+Lemma subst_main M N k : 
+  subst (cbv_cbn M) k (Psi (lam N)) = cbv_cbn (subst M k (lam N)).
+Proof.
+  elim: M k N.
+  - move=> /= n k N. case: (Nat.eqb n k).
+    + done.
+    + done.
+  - move=> s IH1 t IH2 k N /=.
+    rewrite !subst_ren.
+    by rewrite IH1 IH2.
+  - move=> s IH k N /=.
+    rewrite -IH.
+    congr lam. congr app. congr lam.
+    cbn.
+Admitted.
+
+    done.
+    + done.
+    + done. cbn. done. 
+
+Lemma main s t : s ≻ t -> 
+  halt_cbn [] [] (app (cbv_cbn s) (lam (var 0))) -> 
+  halt_cbn [] [] (app (cbv_cbn t) (lam (var 0))).
+Proof.
+  elim; clear s t.
+  - move=> s t /=.
+    do 17 (move=> /halt_cbnE).
+    move=> H'.
+
+  move=> /eval_iff.
+  elim. elim.
+  { admit. }
+
+  move=> > []. 
+
+Lemma test :=
